git réécriture symboles

modélisation Isabelle/sync-mod/SyncModProof.thy
@@ -3,18 +3,18 @@ imports "../HOModel" SyncMod
 begin
 
 definition HOMachine_to_Algorithm :: "(Proc, pstate, SendVal) HOMachine \<Rightarrow> (Proc, pstate, SendVal) CHOAlgorithm" where
-"HOMachine_to_Algorithm mach = \<lparr> CinitState = CinitState mach, sendMsg = sendMsg mach, CnextState = CnextState mach \<rparr>"
+"HOMachine_to_Algorithm mach = (| CinitState = CinitState mach, sendMsg = sendMsg mach, CnextState = CnextState mach |)"
 
 
 definition monovalent :: "(nat \<Rightarrow> Proc \<Rightarrow> pstate proc_state) \<Rightarrow> nat \<Rightarrow> nat \<Rightarrow> bool" where
-"monovalent rho v n \<equiv> \<forall>p ss st. rho n p = Active ss \<longrightarrow> rho (Suc n) p = Active st \<longrightarrow> x st = v"
+"monovalent rho v n \<equiv> !p ss st. rho n p = Active ss \<longrightarrow> rho (Suc n) p = Active st \<longrightarrow> x st = v"
 
 (*lemma A1 : assumes "rho r p = Active s"
 and run:"HORun (HOMachine_to_Algorithm (k_mod.SyncMod_HOMachine k)) rho HO" (is "HORun ?A _ _")
 and "x s = k-1"
-and "p \<in> HO (Suc r) q"
-and "rho r q \<noteq> Aslept"
-shows "\<forall>st. rho (Suc r) q = Active st \<longrightarrow> x st = 0"
+and "p : HO (Suc r) q"
+and "rho r q ~= Aslept"
+shows "!st. rho (Suc r) q = Active st \<longrightarrow> x st = 0"
 proof (rule+)
     fix st
     assume "rho (Suc r) q = Active st"
@@ -24,54 +24,54 @@ proof (rule+)
 lemma stating : assumes "0 < n \<longrightarrow> rho (n-1) p = Aslept"
 and run:"HORun (HOMachine_to_Algorithm (k_mod.SyncMod_HOMachine k)) rho HO" (is "HORun ?A _ _")
 and "rho n p = Active s"
-shows "x s = k" and "\<forall>q. HOrcvdMsgs ?A q (HO (Suc n) q) (rho n) p = (if p \<in> HO (Suc n) q then Content Nope else Void)"
+shows "x s = k" and "!q. HOrcvdMsgs ?A q (HO (Suc n) q) (rho n) p = (if p : HO (Suc n) q then Content Nope else Void)"
 proof -
-    have "CHOinitConfig ?A rho (\<lambda>w ww. undefined)"
-        using run HORun_def[of ?A rho HO] CHORun_def[of ?A rho HO "\<lambda>w ww. undefined"] by simp
+    have "CHOinitConfig ?A rho (%w ww. undefined)"
+        using run HORun_def[of ?A rho HO] CHORun_def[of ?A rho HO "%w ww. undefined"] by simp
     hence "CinitState ?A p s undefined"
-        using CHOinitConfig_def[of ?A rho] \<open>rho n p = Active s\<close> \<open>0 < n \<longrightarrow> rho (n-1) p = Aslept\<close> by auto
+        using CHOinitConfig_def[of ?A rho] `rho n p = Active s` `0 < n \<longrightarrow> rho (n-1) p = Aslept` by auto
     hence "k_mod.SyncMod_initState k p s"
         using HOMachine_to_Algorithm_def by (simp add:k_mod.SyncMod_HOMachine_def)
     hence "x s = k" using k_mod.SyncMod_initState_def[of k p s] by auto
-    hence "\<forall>q. k_mod.SyncMod_sendMsg k p q s = Nope"
+    hence "!q. k_mod.SyncMod_sendMsg k p q s = Nope"
         using k_mod.SyncMod_sendMsg_def[of k p _ s] by fastforce
-    hence "\<forall>q. sendMsg ?A p q s = Nope"
+    hence "!q. sendMsg ?A p q s = Nope"
         using HOMachine_to_Algorithm_def k_mod.SyncMod_HOMachine_def by (simp add: k_mod.SyncMod_HOMachine_def)
-    hence "\<forall>q. HOrcvdMsgs ?A q (HO (Suc n) q) (rho n) p = (if p \<in> HO (Suc n) q then Content Nope else Void)"
+    hence "!q. HOrcvdMsgs ?A q (HO (Suc n) q) (rho n) p = (if p : HO (Suc n) q then Content Nope else Void)"
         using HOrcvdMsgs_def[of ?A p "HO (Suc n) p" "rho n"] by (simp add: HOrcvdMsgs_def assms(3))
-    thus "x s = k" and "\<forall>q. HOrcvdMsgs ?A q (HO (Suc n) q) (rho n) p = (if p \<in> HO (Suc n) q then Content Nope else Void)"
-        using \<open>x s  = k\<close> by auto
+    thus "x s = k" and "!q. HOrcvdMsgs ?A q (HO (Suc n) q) (rho n) p = (if p : HO (Suc n) q then Content Nope else Void)"
+        using `x s  = k` by auto
 qed
 
 lemma sending : assumes run:"HORun (HOMachine_to_Algorithm (k_mod.SyncMod_HOMachine k)) rho HO" (is "HORun ?A rho HO")
 assumes "(HOrcvdMsgs ?A p (HO (Suc (Suc r)) p) (rho (Suc r))) q = Content (Val v)" (is "?msgs q = _")
-shows "\<exists>s ss. rho r q = Active s \<and> rho (Suc r) q = Active ss \<and> x ss = v"
+shows "? s ss. rho r q = Active s \<and> rho (Suc r) q = Active ss \<and> x ss = v"
 proof (cases "rho (Suc r) q")
     case Aslept
-    hence "?msgs q = (if q \<in> HO (Suc (Suc r)) p then Bot else Void)"
+    hence "?msgs q = (if q : HO (Suc (Suc r)) p then Bot else Void)"
         using HOrcvdMsgs_def[of ?A p "HO (Suc (Suc r)) p" "rho (Suc r)"] by auto
-    thus "\<exists>s ss. rho r q = Active s \<and> rho (Suc r) q = Active ss \<and> x ss = v" using \<open>?msgs q = Content (Val v)\<close> by auto
+    thus "? s ss. rho r q = Active s \<and> rho (Suc r) q = Active ss \<and> x ss = v" using `?msgs q = Content (Val v)` by auto
 next
     case (Active sq)
     have "sendMsg ?A q p sq = Val (x sq)"
-        using HOrcvdMsgs_def[of ?A p "HO (Suc (Suc r)) p" "rho (Suc r)"] \<open>?msgs q = Content (Val v)\<close>
+        using HOrcvdMsgs_def[of ?A p "HO (Suc (Suc r)) p" "rho (Suc r)"] `?msgs q = Content (Val v)`
         by (simp add: Active HOMachine_to_Algorithm_def k_mod.SyncMod_HOMachine_def k_mod.SyncMod_sendMsg_def)
     hence "k_mod.SyncMod_sendMsg k q p sq = Val (x sq)"
         using HOMachine_to_Algorithm_def k_mod.SyncMod_HOMachine_def by 
-        (simp add: \<open>\<And>k. k_mod.SyncMod_HOMachine k \<equiv> \<lparr>CinitState = \<lambda>p st crd. k_mod.SyncMod_initState k p st,
-        sendMsg = k_mod.SyncMod_sendMsg k, CnextState = \<lambda>p st msgs crd. k_mod.SyncMod_nextState k p st msgs,
+        (simp add: `\<And>k. k_mod.SyncMod_HOMachine k \<equiv> (|CinitState = %p st crd. k_mod.SyncMod_initState k p st,
+        sendMsg = k_mod.SyncMod_sendMsg k, CnextState = %p st msgs crd. k_mod.SyncMod_nextState k p st msgs,
         HOcommPerRd = k_mod.SyncMod_commPerRd, HOcommGlobal = k_mod.SyncMod_commGlobal,
-        HOcommSchedule = k_mod.SyncMod_commSchedule\<rparr>\<close>)
-    hence "rho r q \<noteq> Aslept"
-        using stating[of "Suc r" rho q k HO sq] \<open>rho (Suc r) q = Active sq\<close>
+        HOcommSchedule = k_mod.SyncMod_commSchedule|)`)
+    hence "rho r q ~= Aslept"
+        using stating[of "Suc r" rho q k HO sq] `rho (Suc r) q = Active sq`
         by (metis SendVal.distinct(1) diff_Suc_1 k_mod.SyncMod_sendMsg_def run)
     then obtain s where "rho r q = Active s" by (cases "rho r q") auto
     moreover have "?msgs q = Content (Val (x sq))"
-        using HOrcvdMsgs_def[of ?A p "HO (Suc (Suc r)) p" "rho (Suc r)"] \<open>?msgs q = Content (Val v)\<close>
-        by (simp add: Active \<open>sendMsg (HOMachine_to_Algorithm (k_mod.SyncMod_HOMachine k)) q p sq = Val (x sq)\<close>)
+        using HOrcvdMsgs_def[of ?A p "HO (Suc (Suc r)) p" "rho (Suc r)"] `?msgs q = Content (Val v)`
+        by (simp add: Active `sendMsg (HOMachine_to_Algorithm (k_mod.SyncMod_HOMachine k)) q p sq = Val (x sq)`)
     ultimately have "rho r q = Active s \<and> rho (Suc r) q = Active sq \<and> x sq = v"
-        using \<open>rho (Suc r) q = Active sq\<close> \<open>?msgs q = Content (Val v)\<close> k_mod.SyncMod_sendMsg_def[of k q p sq] by auto
-    thus "\<exists>s ss. rho r q = Active s \<and> rho (Suc r) q = Active ss \<and> x ss = v"  by auto
+        using `rho (Suc r) q = Active sq` `?msgs q = Content (Val v)` k_mod.SyncMod_sendMsg_def[of k q p sq] by auto
+    thus "? s ss. rho r q = Active s \<and> rho (Suc r) q = Active ss \<and> x ss = v"  by auto
 qed
 
 lemma transition : assumes s_def:"rho r p = Active s"
@@ -81,26 +81,26 @@ and "k > 2"
 shows "k_mod.SyncMod_nextState k p s (HOrcvdMsgs ?A p (HO (Suc r) p) (rho r)) ss" (is "k_mod.SyncMod_nextState  _ _ _ ?msgs _")
 and "x ss < k"
 proof -
-    have "CHOnextConfig ?A (rho r) (HO (Suc r)) (\<lambda>w. undefined) (rho (Suc r))" using run by (simp add:HORun_def CHORun_def)
+    have "CHOnextConfig ?A (rho r) (HO (Suc r)) (%w. undefined) (rho (Suc r))" using run by (simp add:HORun_def CHORun_def)
     then obtain sss where "rho (Suc r) p = Active sss \<and> CnextState ?A p s ?msgs undefined sss" 
-        using CHOnextConfig_def[of ?A "rho r" "HO (Suc r)" "\<lambda>w. undefined" "rho (Suc r)"] s_def by fastforce
+        using CHOnextConfig_def[of ?A "rho r" "HO (Suc r)" "%w. undefined" "rho (Suc r)"] s_def by fastforce
     hence "CnextState ?A p s ?msgs undefined ss" using ss_def by auto
     hence nxt:"k_mod.SyncMod_nextState k p s ?msgs ss"
         using HOMachine_to_Algorithm_def k_mod.SyncMod_HOMachine_def[of k] by (simp add:k_mod.simp_nextState)
     hence "x ss < k"
     proof (cases "k_mod.ready_force k ?msgs s")
         case True
-        thus "x ss < k" using nxt k_mod.SyncMod_nextState_def \<open>k > 2\<close> by auto
+        thus "x ss < k" using nxt k_mod.SyncMod_nextState_def `k > 2` by auto
     next
         case False
         thus "x ss < k"
         proof (cases "x ss = 0")
             case True
-            thus "x ss < k" using \<open>k > 2\<close> by auto
+            thus "x ss < k" using `k > 2` by auto
         next
             case False
             hence "(x ss) mod k = x ss" using nxt k_mod.SyncMod_nextState_def by auto
-            thus "x ss < k" using \<open>k > 2\<close> by (metis less_Suc_eq_0_disj less_imp_Suc_add mod_less_divisor)
+            thus "x ss < k" using `k > 2` by (metis less_Suc_eq_0_disj less_imp_Suc_add mod_less_divisor)
         qed
     qed
     thus "k_mod.SyncMod_nextState k p s ?msgs ss" and "x ss < k" using nxt by auto
@@ -113,7 +113,7 @@ and "x s = k - 1"
 and "k > 2"
 shows "monovalent rho 0 r"
 proof -
-    have "\<forall>p ss st. rho r p = Active ss \<longrightarrow> rho (Suc r) p = Active st \<longrightarrow> x st = 0"
+    have "!p ss st. rho r p = Active ss \<longrightarrow> rho (Suc r) p = Active st \<longrightarrow> x st = 0"
     proof (rule+)
         fix p
         fix ss
@@ -122,42 +122,42 @@ proof -
         assume "rho (Suc r) p = Active st"
         show "x st = 0"
         proof (rule ccontr)
-            assume "x st \<noteq> 0"
+            assume "x st ~= 0"
             let ?msgs = "HOrcvdMsgs ?A p (HO (Suc r) p) (rho r)"
             have "k_mod.SyncMod_sendMsg k xi p s = Val (x s)"
-                using  k_mod.SyncMod_sendMsg_def[of k xi p s] \<open>x s = k - 1\<close> \<open>k > 2\<close> by simp
+                using  k_mod.SyncMod_sendMsg_def[of k xi p s] `x s = k - 1` `k > 2` by simp
             hence "sendMsg ?A xi p s = Val (x s)"
                 using HOMachine_to_Algorithm_def k_mod.SyncMod_HOMachine_def 
-                by (simp add: \<open>\<And>k. k_mod.SyncMod_HOMachine k \<equiv> \<lparr>CinitState = \<lambda>p st crd. k_mod.SyncMod_initState k p st,
-                sendMsg = k_mod.SyncMod_sendMsg k, CnextState = \<lambda>p st msgs crd. k_mod.SyncMod_nextState k p st msgs,
+                by (simp add: `\<And>k. k_mod.SyncMod_HOMachine k \<equiv> (|CinitState = %p st crd. k_mod.SyncMod_initState k p st,
+                sendMsg = k_mod.SyncMod_sendMsg k, CnextState = %p st msgs crd. k_mod.SyncMod_nextState k p st msgs,
                 HOcommPerRd = k_mod.SyncMod_commPerRd, HOcommGlobal = k_mod.SyncMod_commGlobal,
-                HOcommSchedule = k_mod.SyncMod_commSchedule\<rparr>\<close>)
+                HOcommSchedule = k_mod.SyncMod_commSchedule|)`)
             hence "?msgs xi = Content (Val (x s))"
-                using \<open>k_mod.xi_nek HO xi\<close> HOrcvdMsgs_def[of ?A p "HO (Suc r) p" "rho r"] \<open>rho r xi = Active s\<close>
+                using `k_mod.xi_nek HO xi` HOrcvdMsgs_def[of ?A p "HO (Suc r) p" "rho r"] `rho r xi = Active s`
                 k_mod.xi_nek_def[of HO xi] by auto
-            hence "\<not> (k_mod.ready_force k ?msgs ss)"
-                    using k_mod.ready_force_def[of k ?msgs ss] \<open>x s = k-1\<close> by auto
+            hence "~ (k_mod.ready_force k ?msgs ss)"
+                    using k_mod.ready_force_def[of k ?msgs ss] `x s = k-1` by auto
 
             moreover have "CnextState ?A p ss ?msgs undefined st" 
                 using HORun_def CHORun_def run CHOnextConfig_def[of ?A "rho r" _ _ "rho (Suc r)"]
-                \<open>rho r p = Active ss\<close>
-                \<open>rho (Suc r) p = Active st\<close> by fastforce
+                `rho r p = Active ss`
+                `rho (Suc r) p = Active st` by fastforce
             hence "k_mod.SyncMod_nextState k p ss ?msgs st"
                 using HOMachine_to_Algorithm_def k_mod.SyncMod_HOMachine_def[of k]
                 by (simp add: k_mod.simp_nextState)
             ultimately have "k_mod.concordant ?msgs ((x st - 1) mod k)" and "(x st) mod k = x st"
-                using k_mod.SyncMod_nextState_def[of k p ss ?msgs st] \<open>x st \<noteq> 0\<close> 
+                using k_mod.SyncMod_nextState_def[of k p ss ?msgs st] `x st ~= 0` 
                 by auto
-            hence "\<forall>vv. ?msgs xi = Content (Val vv) \<longrightarrow> vv = ((x st - 1) mod k)"
+            hence "!vv. ?msgs xi = Content (Val vv) \<longrightarrow> vv = ((x st - 1) mod k)"
                 using k_mod.concordant_def[of ?msgs "(x st - 1) mod k"] by auto
             hence "k - 1 = (x st - 1) mod k"
-                using \<open>?msgs xi = Content (Val (x s))\<close> \<open>x s = k - 1\<close> by auto
-            hence "(x st) mod k = 0"  using \<open>(x st) mod k = x st\<close>
-                by (smt SendVal.distinct(1) \<open>k_mod.SyncMod_sendMsg k xi p s = Val (x s)\<close>
+                using `?msgs xi = Content (Val (x s))` `x s = k - 1` by auto
+            hence "(x st) mod k = 0"  using `(x st) mod k = x st`
+                by (smt SendVal.distinct(1) `k_mod.SyncMod_sendMsg k xi p s = Val (x s)`
                 add_diff_inverse_nat add_le_cancel_left
                 assms(4) diff_is_0_eq k_mod.SyncMod_sendMsg_def le_add_diff_inverse linorder_not_less
                 mod_by_1 mod_if mod_less_divisor mod_less_eq_dividend nat_code(2))
-            thus "False" using \<open>(x st) mod k = x st\<close> \<open>x st \<noteq> 0\<close> by auto
+            thus "False" using `(x st) mod k = x st` `x st ~= 0` by auto
         qed
     qed
     thus "monovalent rho 0 r" using monovalent_def[of rho 0 r] by auto
@@ -171,11 +171,11 @@ and "k > 2"
 and "monovalent rho (v mod k) r"
 shows "monovalent rho ((v+i) mod k) (r+i)"
 proof (induction i)
-    from assms(6) show \<open>monovalent rho ((v+0) mod k) (r+0)\<close> by auto
+    from assms(6) show `monovalent rho ((v+0) mod k) (r+0)` by auto
 next
     case (Suc i)
     let "?msgs p" = "(HOrcvdMsgs ?A p (HO (Suc (r+Suc i)) p) (rho (r+Suc i)))"
-    have no_discord:"\<forall>p q vv. ?msgs p q = Content (Val vv) \<longrightarrow> vv = (v+i) mod k"
+    have no_discord:"!p q vv. ?msgs p q = Content (Val vv) \<longrightarrow> vv = (v+i) mod k"
     proof (rule+)
         fix p q vv
         assume "?msgs p q = Content (Val vv)"
@@ -185,25 +185,25 @@ next
             using Suc.IH monovalent_def[of rho "(v+i) mod k" "r+i"] by auto
     qed
 
-    have "rho (r+i) xi \<noteq> Aslept"
+    have "rho (r+i) xi ~= Aslept"
         using run HORun_def assms(3) nonAsleepAgain[of rho r xi ?A HO _ i] by (simp add: HORun_def add.commute)
     then obtain sx where "rho (r+i) xi = Active sx" by (cases "rho (r+i) xi") auto
-    moreover have "rho (Suc (r+i)) xi \<noteq> Aslept"
+    moreover have "rho (Suc (r+i)) xi ~= Aslept"
         using run HORun_def assms(3) nonAsleepAgain[of rho r xi ?A HO _ "i+1"] by (simp add: HORun_def add.commute)
     then obtain sxx where "rho (Suc (r+i)) xi = Active sxx" by (cases "rho (Suc (r+i)) xi") auto
     ultimately have "x sxx = (v+i) mod k" using Suc.IH monovalent_def[of rho "(v+i) mod k" "r+i" ] by auto
-    hence "\<forall>p. k_mod.SyncMod_sendMsg k xi p sxx = Val ((v+i) mod k)" using k_mod.SyncMod_sendMsg_def by 
+    hence "!p. k_mod.SyncMod_sendMsg k xi p sxx = Val ((v+i) mod k)" using k_mod.SyncMod_sendMsg_def by 
         (metis One_nat_def add_lessD1 assms(5) linorder_not_less mod_le_divisor mod_less_divisor
         neq0_conv not_add_less2 numerals(2) plus_1_eq_Suc)
-    hence "\<forall>p. sendMsg ?A xi p sxx = Val ((v+i) mod k)"
+    hence "!p. sendMsg ?A xi p sxx = Val ((v+i) mod k)"
         using HOMachine_to_Algorithm_def k_mod.SyncMod_HOMachine_def by (simp add: k_mod.SyncMod_HOMachine_def)
-    hence "\<forall>p. ?msgs p xi = Content (Val ((v+i) mod k))" (is "\<forall>p. ?msgs p xi = _")
-        using assms(1) by (simp add: HOrcvdMsgs_def k_mod.xi_nek_def \<open>rho (Suc (r + i)) xi = Active sxx\<close>)
+    hence "!p. ?msgs p xi = Content (Val ((v+i) mod k))" (is "!p. ?msgs p xi = _")
+        using assms(1) by (simp add: HOrcvdMsgs_def k_mod.xi_nek_def `rho (Suc (r + i)) xi = Active sxx`)
 
-    hence concord:"\<forall>p. k_mod.concordant (?msgs p) ((v+i) mod k)"
+    hence concord:"!p. k_mod.concordant (?msgs p) ((v+i) mod k)"
         using k_mod.concordant_def[of _ "(v+i) mod k"] no_discord by smt
 
-    have "\<forall>p ss st. rho (r+Suc i) p = Active ss \<longrightarrow> rho (Suc (r+Suc i)) p = Active st \<longrightarrow> x st = (v + Suc i) mod k"
+    have "!p ss st. rho (r+Suc i) p = Active ss \<longrightarrow> rho (Suc (r+Suc i)) p = Active st \<longrightarrow> x st = (v + Suc i) mod k"
     proof (rule+)
         fix p ss st
         assume "rho (r+Suc i) p = Active ss" and "rho (Suc (r+Suc i)) p = Active st"
@@ -211,34 +211,34 @@ next
         show "x st = (v + Suc i) mod k"
         proof (cases "k_mod.ready_force k (?msgs p) ss")
             case True
-            hence "\<exists>p1 p2 v1 v2. (?msgs p) p1 = Content (Val v1) \<and> (?msgs p) p2 = Content (Val v2) \<and> v1 \<noteq> v2"
+            hence "? p1 p2 v1 v2. (?msgs p) p1 = Content (Val v1) \<and> (?msgs p) p2 = Content (Val v2) \<and> v1 ~= v2"
                 using k_mod.ready_force_def by blast
             then obtain p1 p2 v1 v2 where "(?msgs p) p1 = Content (Val v1)" and
-                                          "(?msgs p) p2 = Content (Val v2)" and "v1 \<noteq> v2" by auto
+                                          "(?msgs p) p2 = Content (Val v2)" and "v1 ~= v2" by auto
             then obtain s1 s2 ss1 ss2 where "rho (r+i) p1 = Active s1" and "rho (r+Suc i) p1 = Active ss1 \<and> x ss1 = v1" and
                                             "rho (r+i) p2 = Active s2" and "rho (r+Suc i) p2 = Active ss2 \<and> x ss2 = v2"
                 using run sending[of k rho HO p "r+i" p1 v1] sending[of k rho HO p "r+i" p2 v2] by auto
             hence "v1 = (v+i) mod k" and "v2 = (v+i) mod k" using Suc.IH monovalent_def[of rho "(v+i) mod k" "r+i"] by auto
-            thus "x st = (v + Suc i) mod k" using \<open>v1 \<noteq> v2\<close> by auto
+            thus "x st = (v + Suc i) mod k" using `v1 ~= v2` by auto
         next
             case False
             thus "x st = (v + Suc i) mod k"
             proof (cases "x st = 0")
                 case True
-                hence "\<forall>vv. k_mod.concordant (?msgs p) vv \<longrightarrow> vv =  k - 1"
-                    using \<open>k_mod.SyncMod_nextState k p ss (?msgs p) st\<close> k_mod.SyncMod_nextState_def
-                    \<open>\<not> k_mod.ready_force k (?msgs p) ss\<close> by auto
+                hence "!vv. k_mod.concordant (?msgs p) vv \<longrightarrow> vv =  k - 1"
+                    using `k_mod.SyncMod_nextState k p ss (?msgs p) st` k_mod.SyncMod_nextState_def
+                    `~ k_mod.ready_force k (?msgs p) ss` by auto
                 hence "(v+i) mod k = k - 1" using concord k_mod.concordant_def by auto
-                thus "x st = (v+Suc i) mod k" using \<open>x st = 0\<close>
+                thus "x st = (v+Suc i) mod k" using `x st = 0`
                 by (metis Suc_diff_1 assms(5) group_cancel.add2 less_imp_Suc_add mod_Suc_eq mod_self plus_1_eq_Suc zero_less_Suc)
             next
                 case False
                 hence "k_mod.concordant (?msgs p) ((x st - 1) mod k)" and "(x st) mod k = x st"
-                    using \<open>k_mod.SyncMod_nextState k p ss (?msgs p) st\<close> k_mod.SyncMod_nextState_def
-                    \<open>\<not> k_mod.ready_force k (?msgs p) ss\<close> by auto
+                    using `k_mod.SyncMod_nextState k p ss (?msgs p) st` k_mod.SyncMod_nextState_def
+                    `~ k_mod.ready_force k (?msgs p) ss` by auto
                 hence "(x st - 1) mod k = (v+i) mod k"
                     using concord k_mod.concordant_def[of "?msgs p" ] by meson
-                thus "x st = (v+Suc i) mod k" using \<open>(x st) mod k = x st\<close>
+                thus "x st = (v+Suc i) mod k" using `(x st) mod k = x st`
                     by (metis False add_diff_inverse_nat group_cancel.add2 mod_Suc_eq mod_by_1 mod_if plus_1_eq_Suc)
             qed
         qed
@@ -254,8 +254,8 @@ and "k > 2"
 assumes commS:"HOcommSchedule (k_mod.SyncMod_HOMachine k) (Schedule rho)"
 shows "k_mod.liveness rho"
 proof -
-    have "\<exists>n. Schedule rho n = UNIV" using commS by (simp add:k_mod.SyncMod_HOMachine_def k_mod.SyncMod_commSchedule_def )
-    then obtain n :: nat where "!p. rho n p \<noteq> Aslept" by auto
+    have "? n. Schedule rho n = UNIV" using commS by (simp add:k_mod.SyncMod_HOMachine_def k_mod.SyncMod_commSchedule_def )
+    then obtain n :: nat where "!p. rho n p ~= Aslept" by auto
 
     have "monovalent rho 0 r" using A2 assms by auto
     moreover have "(0+(n+1)*k-1) mod k = k-1"
@@ -265,38 +265,38 @@ proof -
         using A3[where ?v = 0 and ?i = "(n+1)*k-1" and ?r = r] assms 
         by (metis (no_types, lifting) add.left_neutral less_one linorder_not_less mod_mult_self1 mod_mult_self2_is_0
         no_zero_divisors not_less0 ordered_cancel_comm_monoid_diff_class.add_diff_assoc zero_eq_add_iff_both_eq_0)
-    have "\<forall>p r. rho r p \<noteq> Aslept --> (\<exists>rf sf. rho rf p = Active sf & fire sf)"
+    have "!p r. rho r p ~= Aslept --> (? rf sf. rho rf p = Active sf & fire sf)"
     proof (rule allI impI)+
         fix p
         fix r :: nat
-        assume "rho r p \<noteq> Aslept"
-        moreover have "1 \<le> (n+1)*k" using \<open>k > 2\<close> by auto
+        assume "rho r p ~= Aslept"
+        moreover have "1 \<le> (n+1)*k" using `k > 2` by auto
         hence "r+((n+1)*k-1) = r+(n+1)*k-1" (is "_ = ?rd") using  ordered_cancel_comm_monoid_diff_class.add_diff_assoc[of 1 "(n+1)*k" r] by auto
-        ultimately have "rho (Suc ?rd) p \<noteq> Aslept" using nonAsleepAgain[of rho r p _ _ _ "(n+1)*k"] run HORun_def
-            by (smt \<open>1 \<le> (n + 1) * k\<close> add.commute add_Suc_right ordered_cancel_comm_monoid_diff_class.add_diff_inverse plus_1_eq_Suc)
+        ultimately have "rho (Suc ?rd) p ~= Aslept" using nonAsleepAgain[of rho r p _ _ _ "(n+1)*k"] run HORun_def
+            by (smt `1 \<le> (n + 1) * k` add.commute add_Suc_right ordered_cancel_comm_monoid_diff_class.add_diff_inverse plus_1_eq_Suc)
         then obtain ss where "rho (Suc ?rd) p = Active ss" by (cases "rho (Suc ?rd) p") auto
-        moreover from this have "rho (Suc (Suc ?rd)) p \<noteq> Aslept"
+        moreover from this have "rho (Suc (Suc ?rd)) p ~= Aslept"
             using nonAsleepAgain[of rho "Suc ?rd" p _ _ _ 1] run HORun_def Suc_diff_1 assms(5) by fastforce
         then obtain st where "rho (Suc (Suc ?rd)) p = Active st" by (cases "rho (Suc (Suc ?rd)) p") auto
         ultimately have "k_mod.SyncMod_nextState k p ss (HOrcvdMsgs ?A p (HO (Suc (Suc ?rd)) p) (rho (Suc ?rd))) st"
             (is "k_mod.SyncMod_nextState  _ _ _ ?msgs _")
             using transition[of rho "Suc ?rd" p ss st] run assms(5) by auto
-        have "\<forall>q. ?msgs p = Void \<or> ?msgs p = Content (Val (k-1))"
+        have "!q. ?msgs p = Void \<or> ?msgs p = Content (Val (k-1))"
         proof
             fix q
-            have "?rd-n = r+n*k+1*k-1-n" using \<open>k > 2\<close> by simp
-            hence positiv:"?rd-n > 0" using \<open>k > 2\<close>
+            have "?rd-n = r+n*k+1*k-1-n" using `k > 2` by simp
+            hence positiv:"?rd-n > 0" using `k > 2`
                 by (metis add.commute add_lessD1 diff_diff_left mult.commute mult.right_neutral mult_less_cancel2
                 one_add_one trans_less_add2 zero_less_diff )
             hence "rho ?rd q ~= Aslept"
-                using nonAsleepAgain[of rho n q ?A HO "\<lambda>r q. undefined" "?rd-n"]
-                run HORun_def[of ?A rho HO] \<open>\<forall>p. rho n p ~= Aslept\<close> \<open>k > 2\<close> by auto
+                using nonAsleepAgain[of rho n q ?A HO "%r q. undefined" "?rd-n"]
+                run HORun_def[of ?A rho HO] `!p. rho n p ~= Aslept` `k > 2` by auto
             then obtain sq where "rho ?rd q = Active sq" by (cases "rho ?rd q") auto
             moreover have "rho (Suc ?rd) q ~= Aslept"
-                using run HORun_def[of ?A rho HO] \<open>k > 2\<close>
-                by (metis \<open>rho ?rd q ~= Aslept\<close> nonAsleepAgain plus_1_eq_Suc)
+                using run HORun_def[of ?A rho HO] `k > 2`
+                by (metis `rho ?rd q ~= Aslept` nonAsleepAgain plus_1_eq_Suc)
             then obtain sqq where "rho (Suc ?rd) q = Active sqq" by (cases "rho (Suc ?rd) q") auto
-            moreover have "r+(n+1)*k > 0" using \<open>k > 2\<close> by auto
+            moreover have "r+(n+1)*k > 0" using `k > 2` by auto
 
 
             moreover have "monovalent rho ((k - 1) :: nat) (?rd :: nat)" using monoval by auto
@@ -307,15 +307,15 @@ proof -
                     using assms monovalent_def[of rho "k-1" ?rd] by auto
 
                 hence "k_mod.SyncMod_sendMsg k q p sqq = Val (k-1)"
-                    using k_mod.SyncMod_sendMsg_def[of k q p sqq] \<open>k > 2\<close> by auto 
+                    using k_mod.SyncMod_sendMsg_def[of k q p sqq] `k > 2` by auto 
                 hence "sendMsg ?A q p sqq = Val (k-1)"
                     using k_mod.SyncMod_HOMachine_def HOMachine_to_Algorithm_def
-                    by (simp add: `\<And>k. k_mod.SyncMod_HOMachine k \<equiv> (| CinitState = \<lambda>p st crd. k_mod.SyncMod_initState k p st,
-                    sendMsg = k_mod.SyncMod_sendMsg k, CnextState = \<lambda>p st msgs crd. k_mod.SyncMod_nextState k p st msgs,
+                    by (simp add: `\<And>k. k_mod.SyncMod_HOMachine k \<equiv> (| CinitState = %p st crd. k_mod.SyncMod_initState k p st,
+                    sendMsg = k_mod.SyncMod_sendMsg k, CnextState = %p st msgs crd. k_mod.SyncMod_nextState k p st msgs,
                     HOcommPerRd = k_mod.SyncMod_commPerRd, HOcommGlobal = k_mod.SyncMod_commGlobal, HOcommSchedule = k_mod.SyncMod_commSchedule |)`)
                 hence "?msgs q = (if q : HO (Suc (Suc ?rd)) p then Content (Val (k-1)) else Void)"
                     using HOrcvdMsgs_def[of ?A p "HO (Suc (Suc ?rd)) p" "rho (Suc ?rd)"] `rho (Suc ?rd) q = Active sqq` by auto
                 thus "?msgs q = Void \<or> ?msgs q = Content (Val (k-1))" by auto
             qed
 
-        show "\<exists>rf sf. rho rf p = Active sf \<and> fire sf"
+        show "? rf sf. rho rf p = Active sf \<and> fire sf"
